common/README.md
@@ -1,0 +1,9 @@
+EasyUC Common Files
+================================================================================
+
+All EasyUC developments should `require` `UCCore.ec`, which consists of
+core UC definitions and lemmas. It `require export`s:
+
+* `UCEncoding.ec` - Encoding and Partial Decoding Pairs (EPDPs)
+
+* `UCUniv.ec` - universe of values (lists of booleans), plus EPDPs
