smc-next/KeysExponentsAndPlainTexts.ec
@@ -1,0 +1,1 @@
+../uc-dsl/examples/smc-case-study/KeysExponentsAndPlainTexts.ec
