uc-dsl/prelude/README.md
@@ -1,0 +1,12 @@
+UC DSL Prelude
+================================================================================
+
+When a UC DSL specification does `ec_requires` and `uc_requires`, this
+prelude directory is always searched first when looking for `.ec`
+and `.uc` files.
+
+The files `UCEncoding.ec` and `UCUniv.ec` are symbolic links to those files
+in `../Common`.
+
+The file `UCCore.ec` is a stripped-down and more abstract version of
+`../common/UCCore.ec`, in which `port` is an abstract type.
